Implement generic total deterministic handler
Fixes #5

theories/Handlers/Deterministic.v
@@ -13,12 +13,15 @@ Section defs.
 
   Variable chain_rule : forall (s : S) (req : req_t), S * ret_t req.
 
-  Inductive det_chain_rule : S -> S -> TE -> Prop :=
-  | det_step : forall s s' pid req ret,
-      (s', ret) = chain_rule s req ->
-      det_chain_rule s s' (trace_elem ctx pid req ret).
+  Definition det_chain_rule (s s' : S) (te : TE) : Prop :=
+    match te with
+    | trace_elem _ _ req ret =>
+      match chain_rule s req with
+      | (s'_, ret_) => s' = s'_ /\ ret = ret_
+      end
+    end.
 
-  Definition t : t :=
+  Definition mkHandler : t :=
     {|
       h_state := S;
       h_req := req_t;
@@ -26,3 +29,188 @@ Section defs.
       h_chain_rule := det_chain_rule;
     |}.
 End defs.
+
+From Coq Require
+     Classes.EquivDec
+     Arith.Peano_dec.
+
+Ltac elim_det H :=
+  match type of H with
+  | ?s = ?s' /\ ?ret = ?ret' =>
+    let Hs := fresh "Hs" in
+    let Hret := fresh "Hret" in
+    destruct H as [Hret Hs];
+    subst s; subst ret;
+    clear H
+  end.
+
+Module AtomicVar.
+  Import EquivDec Peano_dec.
+
+  Section defs.
+    Context {PID T : Set} `{@EqDec T eq eq_equivalence} (init_state : T -> Prop).
+
+    Inductive req_t : Set :=
+    | read : req_t
+    | write : T -> req_t
+    | CAS : T -> T -> req_t.
+
+    Definition ret_t req : Set :=
+      match req with
+      | read => T
+      | write _ => True
+      | CAS _ _ => bool
+      end.
+
+    Definition step s req : T * ret_t req :=
+      match req with
+      | read => (s, s)
+      | write new => (new, I)
+      | CAS old new =>
+        if equiv_dec old s then
+          (new, true)
+        else
+          (s, false)
+      end.
+
+    Definition t := mkHandler PID T req_t ret_t init_state step.
+  End defs.
+
+  Section tests.
+    Let S := nat.
+    Let PID := True.
+    Let Handler := @t PID S eq_nat_dec (fun s => s = 0).
+    Let ctx := hToCtx Handler.
+    Notation "pid '@' ret '<~' req" := (trace_elem ctx pid req ret).
+
+    Goal forall (r1 r2 : S), r1 <> r2 ->
+                        {{fun _ => True}} [I @ r1 <~ read; I @ r2 <~ read] {{fun s => False}}.
+    Proof.
+      intros. unfold_ht.
+      repeat trace_step Hls.
+    Qed.
+  End tests.
+End AtomicVar.
+
+From LibTx Require
+     EqDec
+     Storage.
+
+Module KV.
+  Import Storage EqDec.
+
+  Section defn.
+    (** Parameters:
+    - [PID] type of process id
+    - [K] type of keys
+    - [V] type of values
+    - [S] intance of storage container that should implement [Storage] interface
+    *)
+    Context {PID K V : Set} {S : Set} `{HStore : @Storage K V S} `{HKeq_dec : EqDec K}
+            (init_state : S -> Prop).
+
+    (** ** Syscall types: *)
+    Inductive req_t :=
+    | read : K -> req_t
+    | delete : K -> req_t
+    | write : K -> V -> req_t
+    | snapshot : req_t.
+
+    (** *** Syscall return types: *)
+    Definition ret_t (req : req_t) : Set :=
+      match req with
+      | read _ => option V
+      | delete _ => True
+      | write _ _ => True
+      | snapshot => S
+      end.
+
+    Let ctx := mkCtx PID req_t ret_t.
+    Let TE := @TraceElem ctx.
+
+    Definition step (s : S) (req : req_t) : S * ret_t req :=
+      match req with
+      | read k => (s, get k s)
+      | write k v => (put k v s, I)
+      | delete k => (Storage.delete k s, I)
+      | snapshot => (s, s)
+      end.
+
+    Definition t := mkHandler PID S req_t ret_t init_state step.
+  End defn.
+
+  (** * Properties *)
+  Section Properties.
+    Context {PID K V : Set} {S : Set} `{HStore : @Storage K V S} `{HKeq_dec : EqDec K}
+            {init_state : S -> Prop}.
+
+    Let ctx := mkCtx PID (@req_t K V) (@ret_t K V S).
+    Let TE := @TraceElem ctx.
+
+    Notation "pid '@' ret '<~' req" := (@trace_elem ctx pid req ret).
+
+    (** Two read syscalls always commute: *)
+    Lemma kv_rr_comm : forall p1 p2 k1 k2 v1 v2,
+        @trace_elems_commute_h _ (t init_state) (p1 @ v1 <~ read k1) (p2 @ v2 <~ read k2).
+    Proof.
+      split; intros;
+      repeat trace_step H; subst;
+      repeat forward s';
+      now constructor.
+    Qed.
+
+    (** Read and snapshot syscalls always commute: *)
+    Lemma kv_rs_comm : forall p1 p2 k v s,
+        @trace_elems_commute_h _ (t init_state) (p1 @ v <~ read k) (p2 @ s <~ snapshot).
+    Proof.
+      split; intros;
+      repeat trace_step H; subst;
+      repeat forward s';
+      repeat constructor.
+    Qed.
+
+    Lemma kv_read_get : forall pid (s : h_state (t init_state)) k v,
+        s ~[pid @ v <~ read k]~> s ->
+        v = get k s.
+    Proof.
+      intros.
+      cbn in H.
+      destruct H.
+      now subst.
+    Qed.
+
+    (** Read and write syscalls commute when performed on different keys: *)
+    Lemma kv_rw_comm : forall p1 p2 k1 k2 v1 v2,
+        k1 <> k2 ->
+        @trace_elems_commute_h _ (t init_state) (p1 @ v1 <~ read k1) (p2 @ I <~ write k2 v2).
+    Proof with firstorder.
+      split; intros; repeat trace_step H0.
+      - forward (put k2 v2 s)...
+        forward (put k2 v2 s)...
+        now apply distinct.
+      - forward s...
+        + symmetry. now apply distinct.
+        + forward (put k2 v2 s)...
+    Qed.
+
+    (** Read and delete syscalls commute when performed on different keys: *)
+    Lemma kv_rd_comm : forall p1 p2 k1 k2 v1,
+        k1 <> k2 ->
+        @trace_elems_commute_h _ (t init_state) (p1 @ v1 <~ read k1) (p2 @ I <~ delete k2).
+    Proof with firstorder.
+      split; intros; repeat trace_step H0.
+      - forward (Storage.delete k2 s)...
+        forward (Storage.delete k2 s)...
+        now apply delete_distinct.
+      - forward s...
+        + symmetry. now apply delete_distinct.
+        + forward (Storage.delete k2 s)...
+    Qed.
+
+    (** Write syscalls on different keys generally _don't_ commute! *)
+    Example kv_ww_comm : forall p1 p2 k1 k2 v1 v2,
+        k1 <> k2 ->
+        @trace_elems_commute_h _ (t init_state) (p1 @ I <~ write k1 v1) (p2 @ I <~ write k2 v2).
+    Abort.
+  End Properties.
+End KV.
